Simplified proved_safe_at.

Isabelle2/DistributedSafeAt.thy
@@ -9,127 +9,17 @@ begin
 
 definition acc_max where
   -- {* @{term acc_max} can be computed locally by an acceptor. *}
-  "acc_max a bound \<equiv> 
-    if (\<exists> b < bound . vote a b \<noteq> None)
-    then Some (the_elem (max_by_key (a_votes a bound) snd))
-    else None"
-
-definition a_max where 
-  "a_max b \<equiv> option_as_set o flip acc_max b"
+  "acc_max a bound \<equiv> max_by_key (a_votes a bound) snd"
   
 definition max_quorum_votes where
-  "max_quorum_votes q b \<equiv> max_by_key (\<Union> a \<in> q . a_max b a) snd"
+  "max_quorum_votes q b \<equiv> max_by_key (\<Union> a \<in> q . acc_max a b) snd"
 
 definition proved_safe_at where
   -- {* @{term proved_safe_at} can be computed locally by a leader when it knows acc_max over q *}
   "proved_safe_at q b v \<equiv> q \<in> quorums \<and> (\<forall> a \<in> q . ballot a \<ge> b) \<and>
     v \<in> (fst ` max_quorum_votes q b)"
 
-subsection {* Properties of acc_max. *}
-  
-lemma acc_max_code[code]:
-  fixes get_vote
-  defines "get_vote a b \<equiv> vote a b \<bind> (\<lambda> v . Some (v,b))"
-  shows "acc_max a bound = 
-  (if (\<exists> b < bound . vote a b \<noteq> None)
-  then let votes = (get_vote a ` {0..<bound}) \<bind> option_as_set
-    in Some (the_elem (max_by_key votes snd))
-  else None)"
-proof (cases "\<exists> b < bound . vote a b \<noteq> None")
-  case True
-  then show ?thesis 
-  proof -              
-    have "(get_vote a ` {0..<bound}) \<bind> option_as_set = {(v,b) . b < bound \<and> vote a b = Some v}" 
-      apply (auto simp add:option_as_set_def get_vote_def split!:option.split_asm)
-        apply (simp add: bind_eq_Some_conv)
-       apply (smt bind_eq_Some_conv option.sel prod.inject)
-      by force
-    thus ?thesis
-      by (simp add: distributed_safe_at.acc_max_def) 
-  qed
-next
-  case False
-  then show ?thesis
-    using acc_max_def by auto 
-qed
-
-context begin
-
-private
-lemma a_votes_max: 
-  assumes "b < bound" and "vote a b \<noteq> None"
-  obtains vm bm where "max_by_key (a_votes a bound) snd = {(vm,bm)}"
-proof -
-  obtain x where "max_by_key (a_votes a bound) snd = {x}"
-  proof -
-    have 1:"(a_votes a bound) \<noteq> {}" (is "?votes \<noteq> {}") using assms
-      by (auto simp add:acc_max_def a_votes_def split!: if_split_asm)
-    have 2:"snd x \<noteq> snd y" if "x \<in> (a_votes a bound)" and "y \<in> ?votes" and "x \<noteq> y" for x y
-      using that by (simp add:a_votes_def, case_tac x, case_tac y, auto)
-    show ?thesis using that max_by_key_ordered 1 2 a_votes_finite
-      by (metis (full_types))
-  qed
-  thus ?thesis using that
-    by fastforce 
-qed
-
-lemma acc_max_Some_aux:
-  assumes "acc_max a bound = Some (v,b)"
-  shows "max_by_key (a_votes a bound) snd = {(v,b)}"
-  by (metis (mono_tags, lifting) a_votes_max assms distributed_safe_at.acc_max_def option.sel option.simps(3) the_elem_eq)
-
-lemma acc_max_None:
-  assumes "acc_max a bound = None"
-  shows "max_by_key (a_votes a bound) snd = {}"  using assms
-  using max_by_key[OF a_votes_finite, of a bound snd] 
-  by (auto simp add:acc_max_def a_votes_def split!:if_splits option.splits)
-  
-lemma acc_max_Some_inverse:
-  assumes "acc_max a bound = Some (v,b)" 
-  shows "(v,b) = the_elem (max_by_key (a_votes a bound) snd)"
-    using assms by (simp add:acc_max_def split!:if_splits)
-    
-lemma acc_max_Some:
-  assumes "acc_max a bound = Some (v,b)"
-  shows "vote a b = Some v" and "\<And> b' . \<lbrakk>b' < bound; b < b'\<rbrakk> \<Longrightarrow> vote a b' = None" 
-proof -
-  have 1:"max_by_key (a_votes a bound) snd = {(v,b)}" using acc_max_Some_aux assms by auto
-  have 2:"max_by_key (a_votes a bound) snd = {x \<in> (a_votes a bound) . 
-    \<forall> y \<in> (a_votes a bound) . snd y \<le> snd x}" using max_by_key a_votes_finite by auto
-  show "vote a b = Some v" using 1 2 assms
-    by (auto simp add:a_votes_def)
-  have "(v,b) \<in> a_votes a bound" and "\<And> y . y \<in> a_votes a bound \<Longrightarrow> snd y \<le> b"
-    using 2 by (fastforce simp add:1)+
-  thus "\<And> b' . \<lbrakk>b' < bound; b < b'\<rbrakk> \<Longrightarrow> vote a b' = None" 
-    apply (auto simp add:a_votes_def)
-    by (metis not_less option.collapse)
-qed
-
-lemma acc_max_None_no_vote:
-  assumes "acc_max a bound = None"
-    and "b < bound"
-  shows "vote a b = None"
-  by (metis (no_types, lifting) assms(1) assms(2) distributed_safe_at.acc_max_def option.simps(3))
-
-end
-
-lemma a_max_lemma:"a_max b a = max_by_key (a_votes a b) snd"
-  -- {* Why not use @{term max_by_key} directly instead of wrapping it in an option? 
-  It seems simpler to use a set of votes everywhere, even though we now its a singleton or
-  an empty set. *}
-proof (cases "acc_max a b")
-  case None
-  then show ?thesis
-    apply (simp add:a_max_def option_as_set_def)
-    by (metis distributed_safe_at.acc_max_None)
-next
-  case (Some a)
-  then show ?thesis 
-    apply (simp add:a_max_def option_as_set_def)
-    by (metis distributed_safe_at.acc_max_Some_aux old.prod.exhaust)
-qed
-
-end
+end 
 
 subsection {* Properties of @{term distributed_safe_at.proved_safe_at} *}
 
@@ -137,187 +27,61 @@ locale dsa_properties = quorums quorums + distributed_safe_at quorums ballot vot
   for quorums ballot vote
 begin
 
+sublocale ballot_array_props 
+  by (unfold_locales)
+
 lemma max_quorum_votes:
-  "max_quorum_votes q (flip acc_max b) = 
-  max_by_key {(v,b') . b' < b \<and> (\<exists> a \<in> q . vote a b' = Some v)}  snd"
+  assumes "q \<in> quorums"
+  shows "max_quorum_votes q b =
+  max_by_key {(v,b') . b' < b \<and> (\<exists> a \<in> q . vote a b' = Some v)} snd"
   (is "?lhs = max_by_key ?vs snd")
 proof -
-  let ?vsa = "\<lambda> a . max_by_key {(v,b') . b' < b \<and> vote a b' = Some v} snd"
-  have "Union ((option_as_set o (flip acc_max b)) ` q) = (\<Union>a\<in>q. (?vsa a) )"
-    using acc_max_Some_aux acc_max_None
-    apply (simp add:option_as_set_def split!:option.splits)
-    subgoal proof -
-      fix a :: 'b and ba :: nat and x :: 'a
-      assume a1: "\<And>a bound v b. acc_max a bound = Some (v, b) \<Longrightarrow> max_by_key {(v, b). b < bound \<and> vote a b = Some v} snd = {(v, b)}"
-      assume a2: "x \<in> q"
-      assume a3: "(a, ba) \<in> (case acc_max x b of None \<Rightarrow> {} | Some y \<Rightarrow> {y})"
-      then have "acc_max x b \<noteq> None"
-        by (metis (no_types) empty_iff option.case_eq_if)
-      then have "(a, ba) \<in> max_by_key {(ba, n). n < b \<and> vote x n = Some ba} snd"
-        using a3 a1 by force
-      then show "\<exists>aa\<in>q. (a, ba) \<in> max_by_key {(ba, n). n < b \<and> vote aa n = Some ba} snd"
-        using a2 by blast
-    qed oops
-  
-
-lemma max_vote_unique_aux:
-  assumes "b' < b" and "a \<in> q" and "vote a b' = Some w" and "conservative_array" and "q \<in> quorums"
-  obtains x where "max_quorum_votes q (\<lambda> a . acc_max a b) = {x}"
-proof -
-  let ?votes = "Union ((\<lambda> a . option_as_set ((\<lambda> a . acc_max a b) a)) ` q)"
-  have "finite ?votes" using quorums_axioms apply (simp add:option_as_set_def quorums_def)
-    by (simp add: \<open>q \<in> quorums\<close> option.case_eq_if)
-  have "finite q" using \<open>q \<in> quorums\<close> quorums_axioms
-     by (simp add: quorums_def)
-  have "?votes \<noteq> {}" using assms(1-3) \<open>finite q\<close> acc_max_singleton 
-    apply (auto simp add:option_as_set_def split!:option.splits)
-    using acc_max_def by auto 
-  have "vote a b' = Some v" if "(v,b') \<in> option_as_set (acc_max a b)" for a v b' using that acc_max_is_a_vote
-    by (auto simp add:option_as_set_def split!:option.splits)
-  hence "\<exists> a . vote a b' = Some v" if "(v,b') \<in> ?votes" for v b' using that by blast
-  hence "snd x \<noteq> snd y" if "x \<in> ?votes" and "y \<in> ?votes" and "x \<noteq> y" for x y using \<open>conservative_array\<close> that
-    apply (simp add:conservative_array_def conservative_def split!:option.splits)
-    by (metis old.prod.exhaust snd_conv) 
-  thus ?thesis using that using max_by_key_ordered[where ?f="snd" and ?S="?votes"] \<open>finite ?votes\<close> \<open>?votes \<noteq> {}\<close> 
-    apply (simp add:max_quorum_votes_def) by blast
-qed
-
+  define Ss where "Ss \<equiv> {a_votes a b | a . a \<in> q}"
+  have "finite S" if "S \<in> Ss" for S using that using Ss_def a_votes_finite by blast 
+  moreover
+  have "finite Ss" using \<open>q \<in> quorums\<close> using  quorums_axioms unfolding Ss_def quorums_def  by auto
+  moreover have "{(v, b'). b' < b \<and> (\<exists>a\<in>q. vote a b' = Some v)} = \<Union> Ss"
+    unfolding Ss_def a_votes_def by auto
+  moreover have "(\<Union>a\<in>q. acc_max a b) = (\<Union>S\<in>Ss . max_by_key S snd)" unfolding Ss_def acc_max_def by auto
+  ultimately show ?thesis using max_by_key_subsets[of Ss snd] unfolding max_quorum_votes_def  by auto
+qed 
+ 
 lemma max_vote_unique:
-  -- {* TODO: strengthen this lemma a little bit for the proof of R1 (inv4?) *}
   assumes "conservative_array" and "q \<in> quorums"
-  obtains x where "max_quorum_votes q (\<lambda> a . acc_max a b) = {x}" 
-  | "max_quorum_votes q (\<lambda> a . acc_max a b) = {}"
-proof -
-  have "max_quorum_votes q (flip acc_max b) = {}" if "\<And> a b' . \<lbrakk>a \<in> q; b' < b\<rbrakk> \<Longrightarrow> vote a b' = None" 
-  proof - 
-    note 1 = that
-    let ?maxs="\<Union>x\<in>q. option_as_set (acc_max x b)"
-    have "acc_max a b = None" if "a \<in> q" for a using that 1 by (metis distributed_safe_at.acc_max_def) 
-    hence "?maxs = {}" unfolding option_as_set_def by (metis (mono_tags, lifting) SUP_bot_conv(2) option.case_eq_if) 
-    thus ?thesis unfolding max_quorum_votes_def Let_def  max_by_key_def by auto
-  qed
-  thus ?thesis using that max_vote_unique_aux assms
-    by (metis (full_types) option.exhaust) 
+  obtains x where "max_quorum_votes q b = {x}" 
+  | "max_quorum_votes q b = {}"
+proof (cases "\<exists> a \<in> q . \<exists> b' < b . vote a b' \<noteq> None")
+  case True
+  define vs where "vs \<equiv> q_votes q b"
+  have "vs \<noteq> {}" using True unfolding vs_def q_votes_def by auto
+  moreover have "finite vs" unfolding vs_def
+    by (simp add: assms(2) q_votes_finite) 
+  moreover have "snd x \<noteq> snd y" if "x \<in> vs" and "y \<in> vs" and "x \<noteq> y" for x y 
+    using assms(1) that unfolding vs_def conservative_array_def conservative_def q_votes_def
+    by (auto split!:option.splits) 
+  moreover have "max_quorum_votes q b = max_by_key vs snd" unfolding vs_def q_votes_def
+    by (simp add:max_quorum_votes[OF assms(2)])
+  ultimately
+  obtain x where "max_quorum_votes q b = {x}" using max_by_key_ordered by metis
+  thus ?thesis using that by auto
+next
+  case False
+  then show ?thesis using that max_quorum_votes[OF assms(2)] unfolding max_by_key_def by fastforce
 qed
-  
+
 context begin
 
-private lemma l1:
-  assumes "proved_safe_at q b v"
+private lemma safe_at_imp_safe_at_abs:
+  assumes "proved_safe_at q b v" and "q \<in> quorums"
   shows "proved_safe_at_abs q b v"
-proof -
-  have "v \<in> fst ` (max_by_key {} snd)" if "\<exists> a \<in> q . \<exists> b' < b . vote a b' \<noteq> None" oops
-
-private
-lemma l1: assumes "proved_safe_at q b v" and "conservative_array" shows "proved_safe_at_abs q b v" oops
-nitpick[verbose, card 'a = 3, card nat = 2, card 'b = 3, card "nat option" = 3, card "'b option" = 4, card "('b \<times> nat) option" = 7,
-  card "'b \<times> nat" = 6, expect=none]
-proof -
-  text {* First a few immediate facts. *}
-  from assms have "q \<in> quorums" and bals:"\<And> a . a \<in> q \<Longrightarrow> ballot a \<ge> b" using proved_safe_at_def by auto
-  from \<open>q \<in> quorums\<close> have "finite q" and "q \<noteq> {}"
-    apply (metis quorums_axioms quorums_def) by (metis \<open>q \<in> quorums\<close> empty_iff quorum_inter_witness)
-
-  text {* Re-stating the main goal. *}
-  have "if \<exists> a \<in> q . \<exists> b\<^sub>2 . b\<^sub>2 < b \<and> vote a b\<^sub>2 \<noteq> None
-    then \<exists> a \<in> q . vote a (Max {b\<^sub>2 . \<exists> a \<in> q . b\<^sub>2 < b \<and> vote a b\<^sub>2 \<noteq> None}) = Some v
-    else True" (is "if ?cond then ?true else ?false")
-  proof (cases "?cond")
-    case True    
-    from True obtain a b\<^sub>a where "a \<in> q" and "vote a b\<^sub>a \<noteq> None" and "b\<^sub>a < b" by (auto simp add:acc_max_def)
-    hence "acc_max a b \<noteq> None" by (auto simp add:acc_max_def)
-
-    text {* Using lemma @{thm max_by_key_subsets} *}
-    let ?Ss = "{{(v,b\<^sub>a) . b\<^sub>a < b \<and> vote a b\<^sub>a = Some v} | a . a \<in> q}"
-    let ?S = "{(v,b\<^sub>a) . b\<^sub>a < b \<and> vote a b\<^sub>a = Some v}"
-    have 8:"finite ?Ss" using \<open>finite q\<close> by simp
-    have 9:"\<And> S . S \<in> ?Ss \<Longrightarrow> finite S"
-    proof -
-      { fix S f g
-        assume "finite (f ` S)" and "\<And> x . x \<in> S \<Longrightarrow> x = (g o f) x"
-        hence "finite S" by (metis finite_imageI finite_subset image_comp image_eqI subsetI) }
-      note 1 = this
-      fix S assume "S \<in> ?Ss"
-      obtain a where 2:"S = {(v,b\<^sub>a) . b\<^sub>a < b \<and> vote a b\<^sub>a = Some v}" by (smt \<open>S \<in> ?Ss\<close> mem_Collect_eq)
-      moreover with this have "\<And> x . x \<in> S \<Longrightarrow> x = (the (vote a (snd x)), snd x)" by (metis (mono_tags, lifting) Product_Type.Collect_case_prodD option.sel prod.collapse) 
-      moreover have "finite (snd ` S)" using 2 by (auto simp add:image_def)
-      ultimately show "finite S" using 1[of snd S "\<lambda> b . (the (vote a b), b)"] by (metis comp_def)
-    qed
-    have 5:"?S \<in> ?Ss" using \<open>a \<in> q\<close> by blast
-    have 6:"?S \<noteq> {}" using \<open>b\<^sub>a < b\<close> \<open>vote a b\<^sub>a \<noteq> None\<close> by blast
-    have v_max_max:"v \<in> fst ` (max_by_key (Union {max_by_key S snd | S . S \<in> ?Ss \<and> S \<noteq> {}}) snd)" 
-    proof -
-      let ?acc_maxs_set = "(\<lambda> a . case acc_max a b of None \<Rightarrow> {} | Some (v,b) \<Rightarrow> {(v,b)}) ` q"
-      let ?acc_maxs = "Union ?acc_maxs_set"
-      have 1:"?acc_maxs \<noteq> {}" using \<open>acc_max a b \<noteq> None\<close> apply (auto split add:option.splits) by (metis \<open>a \<in> q\<close>)
-      hence 2:"fst (max_by_key ?acc_maxs snd) = v" using assms(1) proved_safe_at_def 
-        apply (auto simp add:max_quorum_votes_def split add:option.splits) apply (metis option.simps(3)) by (metis (no_types, lifting) fst_conv option.inject) 
-      moreover
-      have 7:"?acc_maxs = {max_by_key S snd | S . S \<in> ?Ss \<and> S \<noteq> {}}"
-        apply (auto simp add: acc_max_def split add:option.splits split_if_asm)
-        apply (smt Collect_empty_eq case_prodI) by (metis (mono_tags) option.simps(3))
-      ultimately show ?thesis by auto 
-    qed
-    hence v_max_Union:"v = fst (max_by_key (Union ?Ss) snd)"
-    proof -
-      have 10:"\<And> x y . \<lbrakk>x \<in> Union ?Ss; y \<in> Union ?Ss; snd x = snd y\<rbrakk> \<Longrightarrow> x = y"
-        using assms(2) by (auto simp add:conservative_array_def conservative_def split:option.splits)
-      show ?thesis using max_by_key_subsets[of ?Ss ?S snd]
-        by (metis (no_types, lifting) "10" "5" "6" "8" "9" v_max_max) 
-    qed
-
-    text {* now we prove that this is the same as Max... *}
-    let ?m = "max_by_key (Union ?Ss) snd"  let ?b\<^sub>m = "snd ?m"
-    have 13:"v = fst ?m" by (metis v_max_Union)
-    let ?bals = "{b\<^sub>2 . b\<^sub>2 < b \<and> (\<exists> a \<in> q . vote a b\<^sub>2 \<noteq> None)}"
-    have bm_max:"?b\<^sub>m = Max ?bals"
-    proof -
-      have "?b\<^sub>m \<in> ?bals" and "\<And> b . b \<in> ?bals \<Longrightarrow> b \<le> ?b\<^sub>m"
-      proof -
-        have 14:"(v,?b\<^sub>m) \<in> Union ?Ss" and 15:"\<And> x . x \<in> Union ?Ss \<Longrightarrow> snd x \<le> ?b\<^sub>m" 
-        proof -
-          have 11:"finite (Union ?Ss)" by (metis (no_types, lifting) "8" "9" finite_Union)
-          have 12:"Union ?Ss \<noteq> {}" by (metis (no_types, lifting) "5" "6" Sup_bot_conv(1))
-          show "(v,?b\<^sub>m) \<in> Union ?Ss" and 15:"\<And> x . x \<in> Union ?Ss \<Longrightarrow> snd x \<le> ?b\<^sub>m"
-            apply (metis (mono_tags, lifting) "11" "12" ex_in_conv max_by_key_in_and_ge(2) surjective_pairing v_max_Union)
-            by (metis (no_types, lifting) "11" max_by_key_in_and_ge(1))
-        qed
-        have 18:"?b\<^sub>m < b" using 14 by auto 
-        have 16:"Union ?Ss = {(v\<^sub>2,b\<^sub>2) . b\<^sub>2 < b \<and> (\<exists> a \<in> q . vote a b\<^sub>2 = Some v\<^sub>2)}" by auto
-        have 17:"\<exists> a \<in> q . vote a ?b\<^sub>m = Some v" and 19:"\<And> b\<^sub>2 v\<^sub>2. b\<^sub>2 < b \<and> (\<exists> a \<in> q . vote a b\<^sub>2 = Some v\<^sub>2) \<Longrightarrow> b\<^sub>2 \<le> ?b\<^sub>m"
-          apply (smt "14" "16" Product_Type.Collect_case_prodD prod.collapse v_max_Union)
-          by (metis (mono_tags, lifting) "15" "16" case_prod_conv mem_Collect_eq snd_conv)
-        show "?b\<^sub>m \<in> ?bals" and "\<And> b . b \<in> ?bals \<Longrightarrow> b \<le> ?b\<^sub>m"
-          apply (metis (mono_tags, lifting) "17" "18" mem_Collect_eq option.simps(3))
-          apply auto apply (insert 19) by (metis (no_types, lifting)) 
-      qed
-      moreover have "finite ?bals" by fastforce
-      moreover have "?bals \<noteq> {}"
-        by (metis (mono_tags, lifting) Collect_empty_eq \<open>a \<in> q\<close> \<open>b\<^sub>a < b\<close> \<open>vote a b\<^sub>a \<noteq> None\<close>) 
-      ultimately show "?b\<^sub>m = Max ?bals" by (metis (no_types, lifting) Max_eqI)
-    qed
-    have m_in_union:"?m \<in> Union ?Ss" 
-    proof -
-      have "finite (Union ?Ss)" by (metis (no_types, lifting) "8" "9" finite_Union) 
-      moreover have "Union ?Ss \<noteq> {}"
-        by (metis (mono_tags, lifting) "5" "6" empty_Union_conv)
-      ultimately show ?thesis by (metis (no_types, lifting) ex_in_conv max_by_key_in_and_ge(2)) 
-    qed
-    obtain a2 where "a2 \<in> q" and max_vote:"vote a2 ?b\<^sub>m = Some v"
-      by (smt Product_Type.Collect_case_prodD UnionE m_in_union mem_Collect_eq v_max_Union) 
-    show ?thesis using bexI[where ?x=a2 and ?A=q] max_vote True \<open>a2 \<in> q\<close> bm_max by auto
-  next
-    case False
-    thus ?thesis by auto
-  qed
-  thus ?thesis using \<open>q \<in> quorums\<close> bals by (auto simp add:proved_safe_at_abs_def)
-qed
+  using  assms unfolding proved_safe_at_def
+  by (simp add:max_quorum_votes[OF assms(2)] proved_safe_at_abs_def)
 
 lemma proved_safe_at_imp_safe_at:
   assumes "\<And> a j w . \<lbrakk>j < i; vote a j = Some w\<rbrakk> \<Longrightarrow> safe_at w j"
-  and "proved_safe_at q i v" and "conservative_array"
-  shows "safe_at v (i::nat)" using l1 ballot_array_props.proved_safe_at_abs_imp_safe_at
-by (metis assms(1) assms(2) assms(3) ballot_array_props.intro quorums_axioms) 
+    and "proved_safe_at q i v" and "conservative_array" and "q \<in> quorums"
+  shows "safe_at v (i::nat)" using safe_at_imp_safe_at_abs assms proved_safe_at_abs_imp_safe_at
+  by blast
 
 end
 
